verif/btrees/index.v
@@ -2,55 +2,21 @@
 
 Require Import Omega.
 
-Inductive index: Type :=
-| im: index
-| ip: Z -> index.
+Definition index := Z.
 
+Definition index_eqb: index -> index -> bool := Z.eqb.
 
-Definition index_eqb (i1:index) (i2:index) : bool :=
-  match i1 with
-  | im => match i2 with
-          | im => true
-          | ip _ => false
-          end
-  | ip n1 => match i2 with
-             | im => false
-             | ip n2 => (Z.eqb n1 n2)
-             end
-  end.
+Definition next_index: index -> index := Z.succ.
 
-Definition next_index (i:index) : index :=
-  match i with
-  | im => ip 0
-  | ip n => ip (Z.succ n)
-  end.
+Definition prev_index: index -> index := Z.pred.
 
-Definition prev_index (i:index) : index :=
-  match i with
-  | im => im
-  | ip n => if Z_le_dec n 0 then im else ip (Z.pred n)
-  end.
+Definition idx_to_Z (i:index) : Z := i.
 
-Definition prev_index_nat (n:Z) : index :=
-  if Z_le_dec n 0 then im else ip (Z.pred n).
-
-Definition index_leb_nat (i:index) (n:Z) : bool :=
-  match i with
-  | im => true
-  | ip n' => (n' <=? n)%Z
-  end.
-
-Definition idx_to_Z (i:index) : Z :=
-  match i with
-  | im => -1
-  | ip n => n
-  end.
+Definition im : index := (-1)%Z.
+Definition ip (i: Z) : index :=  i.
 
 Lemma next_idx_to_Z: forall i,
     (idx_to_Z (next_index i) = (idx_to_Z i) + 1)%Z.
 Proof.
-  intros.
-  destruct i.
-  - simpl. auto.
-  - simpl. omega.
+  intros. reflexivity.
 Qed.
