verif/btrees/verif_isvalid.v
@@ -28,7 +28,7 @@ Proof.
   simpl in H0. contradiction.          (* the empty cursor can't be complete *)
   pose (c:=(n,i)::c'). fold c.
   assert (n = currNode c r). simpl. auto.
-  simpl in H0. destruct i as [|ii]. contradiction.
+  simpl in H0.
   apply complete_cursor_subnode in H. unfold get_root in H. simpl in H.
   assert (SUBNODE: subnode n root) by auto.
   unfold relation_rep. unfold r.
@@ -63,22 +63,24 @@ Proof.
       * forward.                (* t'3=(tbool) (t'6==1) *)
         entailer!.
         { unfold isValid. rewrite H4. destruct Last; simpl; auto.
-          assert (Hii: 0 <= ii < numKeys_le le). {
+          assert (Hii: 0 <= i < numKeys_le le). {
                clear - COMPLETE H4 H3. rewrite H3,H4 in COMPLETE.
                clear H3 H4. destruct COMPLETE. hnf in H. simpl in H.
-               destruct (nth_entry_le ii le) eqn:?H; try contradiction.
-               apply nth_entry_le_some  in H1. auto.
+               if_tac in H; try contradiction.
+               destruct (nth_entry_le i le) eqn:?H; try contradiction.
+               apply nth_entry_le_some  in H2. auto.
           }
           assert(0 <= numKeys_le le <= Int.max_unsigned).
           { apply H1 in SUBNODE. apply node_wf_numKeys in SUBNODE. unfold numKeys in SUBNODE.
             rewrite H3 in SUBNODE. rewrite H4 in SUBNODE. rep_omega. }
-          apply repr_inj_unsigned in H5.
+          apply repr_inj_unsigned in H5. unfold index_eqb, ip. unfold rep_index, idx_to_Z in H5.
           rewrite H5. rewrite Z.eqb_refl. auto.
           unfold complete_cursor in COMPLETE. destruct COMPLETE.
           unfold complete_cursor_correct_rel in H16.
-          destruct (getCEntry ((n,ip ii)::c')); try inv H16.
+          destruct (getCEntry ((n,i)::c')); try inv H16.
           destruct e; try inv H16.
           apply complete_correct_index in H16. rewrite H3, H4 in H16. simpl in H16.
+          unfold rep_index, idx_to_Z.
           rep_omega. auto. }
         rewrite unfold_btnode_rep. rewrite H4.
         entailer!. Exists ent_end0. entailer!. fold r. cancel.
@@ -122,7 +124,6 @@ Proof.
   { simpl in H0. contradiction. } (* the empty cursor can't be complete *)
   pose (c:=(n,i)::c'). fold c.
   assert (n = currNode c r). simpl. auto.
-  simpl in H0. destruct i as [|ii]. contradiction. 
   apply complete_cursor_subnode in H. unfold get_root in H. simpl in H.
   assert (SUBNODE: subnode n root) by auto.
   unfold c. simpl. fold c.
@@ -130,8 +131,8 @@ Proof.
   pose (n:=btnode val ptr0 le isLeaf First Last pn). fold n in c, H3, SUBNODE, COMPLETE.
   forward_if(
       PROP ( )
-      LOCAL (temp _t'1 (Vint (Int.repr ii)); temp _cursor pc;
-             temp _t'2 (Val.of_bool(First && (index_eqb (ip ii) (ip 0))))) (* new local *)
+      LOCAL (temp _t'1 (Vint (Int.repr i)); temp _cursor pc;
+             temp _t'2 (Val.of_bool(First && (index_eqb i (ip 0))))) (* new local *)
       SEP (malloc_token Ews trelation prel *
            data_at Ews trelation
            (getval root,
@@ -146,14 +147,15 @@ Proof.
     forward.                    (* t'4=t'3->First *)
     { destruct First; entailer!. }
     forward.                    (* t'2=(t'4==1) *)
-    assert(ii=0).
+    assert(i=0).
     { unfold complete_cursor in COMPLETE. destruct COMPLETE.
     unfold complete_cursor_correct_rel in H5.
-    destruct( getCEntry ((n,ip ii)::c')) eqn:?H; try contradiction.
-    simpl in H7. apply nth_entry_le_some in H7.
+    destruct( getCEntry ((n,i)::c')) eqn:?H; try contradiction.
+    simpl in H7. if_tac in H7. inv H7. apply nth_entry_le_some in H7.
     apply H1 in SUBNODE. apply node_wf_numKeys in SUBNODE.
     unfold n in SUBNODE. simpl in SUBNODE.
     apply (f_equal Int.unsigned) in H4.
+    unfold rep_index, idx_to_Z in H4.
     rewrite !Int.unsigned_repr in H4 by rep_omega. auto. } subst.
     sep_apply (fold_btnode_rep ptr0). fold n.
     sep_apply modus_ponens_wand.
@@ -163,7 +165,7 @@ Proof.
   - Intros.
     forward.                    (* t'2=0 *)
     entailer!.
-    simpl. rewrite (proj2 (Z.eqb_neq ii 0)). rewrite andb_comm. reflexivity.
+    simpl. unfold index_eqb. rewrite (proj2 (Z.eqb_neq i 0)). rewrite andb_comm. reflexivity.
     contradict H4; f_equal; auto. 
   - forward_if.
     + forward.                  (* return 1 *)
