verif/btrees/verif_splitnode_part0.v
@@ -101,16 +101,18 @@ Proof.
   - simpl. if_tac; auto.
   - simpl in *.
      destruct e0.
-    + simpl. destruct (k_ (entry_key e) <=? k_ k) eqn:?H. inv H0.
+    + simpl. destruct (k_ (entry_key e) <=? k_ k) eqn:?H;
+        unfold ip in *; subst.
         rewrite Z.sub_diag. simpl. auto.
-        pose proof (FRI_increase X le (entry_key e) (ip (Z.succ i))). rewrite <- H0 in H2.
-        simpl in H2. rewrite !zle_false by omega. simpl.
+        pose proof (FRI_increase X le (entry_key e) (Z.succ i)).
+        unfold idx_to_Z, next_index in *. rewrite !zle_false by omega. simpl.
        f_equal. rewrite (IHle (Z.succ i)); auto; try omega.
        f_equal. f_equal. omega. f_equal. f_equal. omega.
-    + simpl. destruct (k_ (entry_key e) <=? k_ k) eqn:?H. inv H0.
+    + simpl. destruct (k_ (entry_key e) <=? k_ k) eqn:?H;
+        unfold ip in *; subst.
         rewrite Z.sub_diag. simpl. auto.
-        pose proof (FRI_increase X le (entry_key e) (ip (Z.succ i))). rewrite <- H0 in H2.
-        simpl in H2. rewrite !zle_false by omega. simpl.
+        pose proof (FRI_increase X le (entry_key e) (Z.succ i)).
+        unfold idx_to_Z, next_index in *. rewrite !zle_false by omega. simpl.
        f_equal. rewrite (IHle (Z.succ i)); auto; try omega.
        f_equal. f_equal. omega. f_equal. f_equal. omega.
 Qed.
@@ -185,24 +187,24 @@ Lemma nth_first_insert: forall X (le:listentry X) e k m,
 Proof.
   intros. subst.
   generalize dependent m. induction le; intros.
-  - simpl in H0. simpl. rewrite !zle_true by omega. auto.
+  - simpl in H0. unfold idx_to_Z,ip in H0. simpl. rewrite !zle_true by omega. auto.
   - simpl. simpl in H0. destruct e0.
     + simpl. destruct (k_ (entry_key e) <=? k_ k).
-      * simpl in H0. assert (m=0) by omega; subst m; simpl; auto.
+      * simpl in H0. unfold idx_to_Z, ip in *.
+         assert (m=0) by omega; subst m; simpl; auto.
       * if_tac. assert (m=0) by omega. subst; simpl; auto.
+         unfold idx_to_Z, ip in *.
          simpl. rewrite zle_false by omega. f_equal. apply IHle.
-         pose proof (FRI'_next_index le (entry_key e) (ip 0)). simpl in H1.
-         rewrite H1 in H0.
-         destruct ((findRecordIndex' le (entry_key e) (ip 0))). simpl in H0. omega.
-         simpl in *. omega.
+         pose proof (FRI'_next_index le (entry_key e) 0). simpl in H1.
+         unfold next_index in *. omega.
     + simpl. destruct (k_ (entry_key e) <=? k_ k).
-      * simpl in H0. assert (m=0) by omega; subst m; simpl; auto.
+      * simpl in H0.  unfold idx_to_Z, ip in *.
+         assert (m=0) by omega; subst m; simpl; auto.
       * if_tac. assert (m=0) by omega. subst; simpl; auto.
          simpl. rewrite zle_false by omega. f_equal. apply IHle.
-         pose proof (FRI'_next_index le (entry_key e) (ip 0)). simpl in H1.
-         rewrite H1 in H0.
-         destruct ((findRecordIndex' le (entry_key e) (ip 0))). simpl in H0. omega.
-         simpl in *. omega.
+         unfold idx_to_Z, ip in *.
+         pose proof (FRI'_next_index le (entry_key e) 0). simpl in H1.
+         rewrite H1 in H0. unfold next_index in *. omega.
 Qed.
 
 Lemma nth_first_app_same1: forall X (le1:listentry X) le2 i,
