verif/btrees/verif_splitnode_part2.v
@@ -106,9 +106,9 @@ Proof.
     assert(LEAF: isLeaf=true).
     { destruct isLeaf; auto. simpl in H2. inv H2. }
    clear H2; pose (H2:=True).
-    destruct (findRecordIndex n k) as [|fri] eqn:HFRI.
-    { simpl in INRANGE. omega. }
-    replace (findRecordIndex' le k (index.ip 0)) with (index.ip fri). simpl.
+    remember (findRecordIndex n k) as fri eqn:HFRI.
+    unfold idx_to_Z, ip in *. 
+    replace (findRecordIndex' le k 0) with fri. simpl.
     change (Vint (Int.repr 0)) with (Val.of_bool false).
     sep_apply (fold_btnode_rep ptr0). 
      rewrite LEAF.
@@ -133,8 +133,6 @@ Proof.
       SEP (mem_mgr gv; btnode_rep nleft; btnode_rep (empty_node isLeaf false Last vnewnode);
            data_at Tsh (tarray tentry 16) (le_to_list (nth_first_le le i)++ allent_end) v_allEntries;
            entry_rep e; data_at Ews tentry (keyrepr, coprepr) pe)))%assert.
-    { simpl in INRANGE; rep_omega. }
-    { simpl in INRANGE; rep_omega. }
     { entailer!.
       Exists (default_val (nested_field_type (tarray (Tstruct _Entry noattr) 16) [])).
       entailer!. unfold data_at_, field_at_. simpl.
@@ -179,7 +177,7 @@ Proof.
           rewrite sublist_same by omega. simpl in H4. rewrite Zlength_cons in *. rep_omega. }
       assert(INUM: i <= numKeys_le le).
       { unfold n  in H0. simpl in H0. rewrite H0. clear -INRANGE H3.
-        simpl in INRANGE. rep_omega.  }
+        simpl in INRANGE. change (findRecordIndex' le k (ip 0)) with (findRecordIndex n k) in *; rep_omega.  }
       rewrite unfold_btnode_rep with (n:=nleft). unfold nleft. Exists ent_end. cancel.      
       rewrite upd_Znth_twice.
       rewrite app_Znth2. rewrite le_to_list_length. rewrite numKeys_nth_first.
@@ -212,6 +210,7 @@ Proof.
     rewrite ENTRY in HEVR. simpl in HEVR. inv HEVR.
 
     Opaque Znth.
+    set (fri := findRecordIndex n k) in *.
     forward.                    (* allEntries[tgtIdx]->key = t'24 *)
     apply prop_right; rep_omega.
     forward.                    (* t'23=entry->ptr.record *)
@@ -283,6 +282,7 @@ Proof.
       rewrite upd_Znth_twice.
       (* rewrite upd_Znth_app2. *)
       rewrite upd_Znth_same.
+      set (fri := findRecordIndex n k) in *.
       assert((upd_Znth (i + 1) (le_to_list (nth_first_le le fri) ++ (Vptrofs (Ptrofs.repr (k_ k)), inr xe) :: le_to_list (suble (fri) i le) ++ x) (key_repr ki, inr xi)) = (le_to_list (nth_first_le le fri) ++ (Vptrofs (Ptrofs.repr (k_ k)), inr xe) :: le_to_list (suble fri (i + 1) le) ++ sublist 1 (Zlength x) x)).
       { rewrite upd_Znth_app2. rewrite le_to_list_length. rewrite numKeys_nth_first.
         change (?A::?B) with ([A]++B).
@@ -323,6 +323,7 @@ Proof.
     change Delta with (func_tycontext f_splitnode Vprog Gprog []).
     subst POSTCONDITION; unfold abbreviate.
     clear MORE_COMMANDS.
-    clear - FRILENGTH H4 H5 FRIRANGE H3 PTRXE H1 INRANGE HFRI H H0 LEAFENTRY.
-    eapply splitnode_main_if_part2_proof; eassumption.
+    clear - FRILENGTH H4 H5 FRIRANGE H3 PTRXE H1 INRANGE H H0 LEAFENTRY.
+    eapply splitnode_main_if_part2_proof; try eassumption.
+    reflexivity.
 Qed.
